compiler/backend/semantics/bvpPropsScript.sml
@@ -461,6 +461,15 @@ val bvp_to_bvi_ignore = Q.store_thm("bvp_to_bvi_ignore",
    (bvp_to_bvi (s with <| locals := l; space := t |>) = bvp_to_bvi s)`,
   EVAL_TAC);
 
+val bvp_to_bvi_refs = Q.store_thm("bvp_to_bvi_refs",
+  `bvp_to_bvi (s with refs := r) = bvp_to_bvi s with refs := r`,
+  EVAL_TAC);
+
+val bvi_to_bvp_refs = Q.store_thm("bvi_to_bvp_refs",
+  `((bvi_to_bvp s t with refs := z) = bvi_to_bvp (s with refs := z) t) /\
+   ((bvi_to_bvp s t).refs = s.refs)`,
+  EVAL_TAC);
+
 val bvi_to_bvp_space_locals = Q.store_thm("bvi_to_bvp_space_locals",
   `((bvi_to_bvp s t with locals := x) = bvi_to_bvp s (t with locals := x)) /\
    ((bvi_to_bvp s t).locals = t.locals) /\
